theories/SimGlobal.v
@@ -24,15 +24,15 @@ Variable ord: idx -> idx -> Prop.
 Hypothesis wf_ord: well_founded ord.
 
 Section TY.
-Context `{R: Type}.
-Inductive _simg (simg: idx -> relation (itree eventE R)) (i0: idx): relation (itree eventE R) :=
+(* Context `{R: Type}. *)
+Inductive _simg (simg: forall R, idx -> relation (itree eventE R)) {R} (i0: idx): relation (itree eventE R) :=
 | simg_ret
     r
   :
     _simg simg i0 (Ret r) (Ret r)
 | simg_syscall
     i1 ktr_src0 ktr_tgt0 fn m0 varg
-    (SIM: (eq ==> simg i1)%signature ktr_src0 ktr_tgt0)
+    (SIM: (eq ==> simg _ i1)%signature ktr_src0 ktr_tgt0)
   :
     _simg simg i0 (trigger (Syscall fn m0 varg) >>= ktr_src0) (trigger (Syscall fn m0 varg) >>= ktr_tgt0)
 
@@ -40,19 +40,19 @@ Inductive _simg (simg: idx -> relation (itree eventE R)) (i0: idx): relation (it
 
 | simg_tau
     i1 itr_src0 itr_tgt0
-    (SIM: simg i1 itr_src0 itr_tgt0)
+    (SIM: simg _ i1 itr_src0 itr_tgt0)
   :
     _simg simg i0 (tau;; itr_src0) (tau;; itr_tgt0)
 | simg_tauL
     i1 itr_src0 itr_tgt0
     (ORD: ord i1 i0)
-    (SIM: simg i1 itr_src0 itr_tgt0)
+    (SIM: simg _ i1 itr_src0 itr_tgt0)
   :
     _simg simg i0 (tau;; itr_src0) (itr_tgt0)
 | simg_tauR
     i1 itr_src0 itr_tgt0
     (ORD: ord i1 i0)
-    (SIM: simg i1 itr_src0 itr_tgt0)
+    (SIM: simg _ i1 itr_src0 itr_tgt0)
   :
     _simg simg i0 (itr_src0) (tau;; itr_tgt0)
 
@@ -60,19 +60,19 @@ Inductive _simg (simg: idx -> relation (itree eventE R)) (i0: idx): relation (it
 
 | simg_choose
     i1 X_src X_tgt ktr_src0 ktr_tgt0
-    (SIM: forall x_tgt, exists x_src, simg i1 (ktr_src0 x_src) (ktr_tgt0 x_tgt))
+    (SIM: forall x_tgt, exists x_src, simg _ i1 (ktr_src0 x_src) (ktr_tgt0 x_tgt))
   :
     _simg simg i0 (trigger (Choose X_src) >>= ktr_src0) (trigger (Choose X_tgt) >>= ktr_tgt0)
 | simg_chooseL
     i1 X ktr_src0 itr_tgt0
     (ORD: ord i1 i0)
-    (SIM: exists x, simg i1 (ktr_src0 x) itr_tgt0)
+    (SIM: exists x, simg _ i1 (ktr_src0 x) itr_tgt0)
   :
     _simg simg i0 (trigger (Choose X) >>= ktr_src0) (itr_tgt0)
 | simg_chooseR
     i1 X itr_src0 ktr_tgt0
     (ORD: ord i1 i0)
-    (SIM: forall x, simg i1 itr_src0 (ktr_tgt0 x))
+    (SIM: forall x, simg _ i1 itr_src0 (ktr_tgt0 x))
   :
     _simg simg i0 (itr_src0) (trigger (Choose X) >>= ktr_tgt0)
 
@@ -80,26 +80,26 @@ Inductive _simg (simg: idx -> relation (itree eventE R)) (i0: idx): relation (it
 
 | simg_take
     i1 X_src X_tgt ktr_src0 ktr_tgt0
-    (SIM: forall x_src, exists x_tgt, simg i1 (ktr_src0 x_src) (ktr_tgt0 x_tgt))
+    (SIM: forall x_src, exists x_tgt, simg _ i1 (ktr_src0 x_src) (ktr_tgt0 x_tgt))
   :
     _simg simg i0 (trigger (Take X_src) >>= ktr_src0) (trigger (Take X_tgt) >>= ktr_tgt0)
 | simg_takeL
     i1 X ktr_src0 itr_tgt0
     (ORD: ord i1 i0)
-    (SIM: forall x, simg i1 (ktr_src0 x) itr_tgt0)
+    (SIM: forall x, simg _ i1 (ktr_src0 x) itr_tgt0)
   :
     _simg simg i0 (trigger (Take X) >>= ktr_src0) (itr_tgt0)
 | simg_takeR
     i1 X itr_src0 ktr_tgt0
     (ORD: ord i1 i0)
-    (SIM: exists x, simg i1 itr_src0 (ktr_tgt0 x))
+    (SIM: exists x, simg _ i1 itr_src0 (ktr_tgt0 x))
   :
     _simg simg i0 (itr_src0) (trigger (Take X) >>= ktr_tgt0)
 .
 
-Definition simg: idx -> relation (itree eventE R) := paco3 _simg bot3.
+Definition simg: forall R, idx -> relation (itree eventE R) := paco4 _simg bot4.
 
-Lemma simg_mon: monotone3 _simg.
+Lemma simg_mon: monotone4 _simg.
 Proof.
   ii. inv IN; try (by econs; et).
   - econs; et. ii. eapply LE; et.
@@ -110,8 +110,142 @@ Proof.
 Qed.
 End TY.
 
+Hint Constructors _simg.
+Hint Unfold simg.
+Hint Resolve simg_mon: paco.
+
+
 
 (*** TODO: for bind rule, take a look at "respectful" thing again. ***)
+Variable add: idx -> idx -> idx.
+Variant bindR (r s: forall S, idx -> relation (itree eventE S)): forall S, idx -> relation (itree eventE S) :=
+| bindR_intro
+    o0 o1
+
+    R
+    (i_src i_tgt: itree eventE R)
+    (SIM: simg o0 i_src i_tgt)
+
+    S
+    (k_src k_tgt: ktree eventE R S)
+    (SIMK: forall (vret: R), simg o1 (k_src vret) (k_tgt vret))
+  :
+    bindR r s (add o0 o1) (ITree.bind i_src k_src) (ITree.bind i_tgt k_tgt)
+.
+
+Hint Constructors bindR: core.
+
+Lemma bindR_mon
+      r1 r2 s1 s2
+      (LEr: r1 <4= r2) (LEs: s1 <4= s2)
+  :
+    bindR r1 s1 <4= bindR r2 s2
+.
+Proof. ii. destruct PR; econs; et. Qed.
+
+Definition bindC r := bindR r r.
+Hint Unfold bindC: core.
+
+(* Lemma bindC_wrespectful: wrespectful4 (_sim_st lt) bindC. *)
+(* Proof. *)
+(*   econstructor; repeat intro. *)
+(*   { eapply bindR_mon; eauto. } *)
+(*   rename l into llll. *)
+(*   eapply bindR_mon in PR; cycle 1. *)
+(*   { eapply GF. } *)
+(*   { i. eapply PR0. } *)
+(*   inv PR. csc. inv SIM. *)
+(*   + irw. *)
+(*     exploit SIMK; eauto. i. *)
+(*     eapply sim_st_mon_ord. *)
+(*     { instantiate (1:=i1). rewrite rtc_lt. lia. } *)
+(*     eapply sim_st_mon; eauto with paco. *)
+(*   + irw. econs; eauto. *)
+(*     { econs 2; eauto with paco. econs; eauto with paco. ii. exploit SIMK; eauto with paco. } *)
+(*   + irw. econs; eauto. *)
+(*     { econs 2; eauto with paco. econs; eauto with paco. ii. exploit SIMK; eauto with paco. } *)
+(*   + irw. econs; eauto. *)
+(*   + irw. econs; eauto. *)
+(*   + irw. econs; eauto. *)
+(*     { ii. spc SIM0. des. esplits; eauto. *)
+(*       econs 2; eauto with paco. econs; eauto with paco. ii. exploit SIMK; eauto with paco. } *)
+(*   + irw. des. econs; eauto. *)
+(*     { esplits; eauto. *)
+(*       econs 2; eauto with paco. econs; eauto with paco. ii. exploit SIMK; eauto with paco. } *)
+(*     { rewrite tc_lt in *. lia. } *)
+(*   + irw. econs; eauto. ii. spc SIM0. des. esplits; eauto. *)
+(*     { econs 2; eauto with paco. econs; eauto with paco. ii. exploit SIMK; eauto with paco. } *)
+(*     { rewrite tc_lt in *. lia. } *)
+(*   + irw. econs; eauto. *)
+(*     { econs 2; eauto with paco. econs; eauto with paco. ii. exploit SIMK; eauto with paco. } *)
+(*     { rewrite tc_lt in *. lia. } *)
+(*   + irw. econs; eauto. *)
+(*     { econs 2; eauto with paco. econs; eauto with paco. ii. exploit SIMK; eauto with paco. } *)
+(*     { rewrite tc_lt in *. lia. } *)
+(*   + irw. econs; eauto. *)
+(*     { econs 2; eauto with paco. econs; eauto with paco. ii. exploit SIMK; eauto with paco. } *)
+(*   + irw. econs; eauto. *)
+(*     { econs 2; eauto with paco. econs; eauto with paco. ii. exploit SIMK; eauto with paco. } *)
+(*     { rewrite tc_lt in *. lia. } *)
+(*   + irw. econs; eauto. *)
+(*     { econs 2; eauto with paco. econs; eauto with paco. ii. exploit SIMK; eauto with paco. } *)
+(*     { rewrite tc_lt in *. lia. } *)
+(*   + irw. econs; eauto. *)
+(*     { econs 2; eauto with paco. econs; eauto with paco. ii. exploit SIMK; eauto with paco. } *)
+(*   + irw. econs; eauto. *)
+(*     { econs 2; eauto with paco. econs; eauto with paco. ii. exploit SIMK; eauto with paco. } *)
+(*     { rewrite tc_lt in *. lia. } *)
+(*   + irw. econs; eauto. *)
+(*     { econs 2; eauto with paco. econs; eauto with paco. ii. exploit SIMK; eauto with paco. } *)
+(*     { rewrite tc_lt in *. lia. } *)
+(* Qed. *)
+
+(* Lemma bindC_spec: bindC <5= gupaco4 (_sim_st lt) (cpn4 (_sim_st lt)). *)
+(* Proof. *)
+(*   intros. eapply wrespect4_uclo; eauto with paco. eapply bindC_wrespectful. *)
+(* Qed. *)
+
+
+
+
+
+
+(* Lemma bindC_spec *)
+(*       simC *)
+(*   : *)
+(*     bindC <5= gupaco4 (_simg) (simC) *)
+(* . *)
+(* Proof. *)
+(*   gcofix CIH. intros. destruct PR. *)
+(*   punfold SIM. inv SIM. *)
+(*   - irw. gbase. eapply SIMK; et. rewrite ! bind_ret_l. gbase. eapply SIMK; et. rr; et. *)
+(*   - rewrite ! bind_tau. gstep. econs; eauto. pclearbot. *)
+(*     (* gfinal. left. eapply CIH. econstructor; eauto. *) *)
+(*     debug eauto with paco. *)
+(*   - rewrite ! bind_vis. gstep. econs; eauto. u. ii. repeat spc MATCH. pclearbot. eauto with paco. *)
+(*   - rewrite ! bind_vis. gstep. econs; eauto. u. ii. repeat spc MATCH. pclearbot. *)
+(*     eauto with paco. *)
+(*   - rewrite ! bind_vis. gstep. econs; eauto. *)
+(*   - rewrite ! bind_vis. gstep. econs; eauto. *)
+(*   - rewrite ! bind_vis. *)
+(*     gstep. econs; eauto. ii. exploit SIM0; et. intro T; des_safe. pclearbot. eauto with paco. *)
+(*   - rewrite ! bind_vis. rewrite ! bind_tau. *)
+(*     gstep. econs; eauto. des. pclearbot. eauto with paco. *)
+(*   - rewrite ! bind_vis. rewrite ! bind_tau. *)
+(*     gstep. econs; eauto. ii. pclearbot. eauto with paco. *)
+(* Qed. *)
+
+(* Global Instance match_itr_bind : *)
+(*   HProper ((SALL !-> match_itr) !-> match_itr !-> match_itr) ITree.bind' ITree.bind' *)
+(* . *)
+(* Proof. *)
+(*   red. ginit. *)
+(*   { intros. eapply cpn2_wcompat; eauto with paco. } *)
+(*   guclo bindC_spec. ii. econs; et. *)
+(*   u. ii. *)
+(*   exploit H0; et. *)
+(*   intro T. eauto with paco. *)
+(* Qed. *)
 
 
 
@@ -123,16 +257,17 @@ Definition resum_itr E F `{E -< F}: itree E ~> itree F := fun _ itr => interp (f
 Variable md_src md_tgt: Mod.t.
 Let ms_src: ModSem.t := md_src.(Mod.enclose).
 Let ms_tgt: ModSem.t := md_tgt.(Mod.enclose).
-Let sim_fnsem: relation (string * (list val -> itree Es val)) :=
-  fun '(fn_src, fsem_src) '(fn_tgt, fsem_tgt) =>
-    (<<NAME: fn_src = fn_tgt>>) /\
-    (<<SEM: forall varg, exists itr_src itr_tgt,
-          (<<SRC: fsem_src varg = resum_itr itr_src>>) /\
-          (<<TGT: fsem_tgt varg = resum_itr itr_tgt>>) /\
-          (<<SIM: exists i0, simg i0 itr_src itr_tgt>>)>>)
-.
+(* Let sim_fnsem: relation (string * (list val -> itree Es val)) := *)
+(*   fun '(fn_src, fsem_src) '(fn_tgt, fsem_tgt) => *)
+(*     (<<NAME: fn_src = fn_tgt>>) /\ *)
+(*     (<<SEM: forall varg, exists itr_src itr_tgt, *)
+(*           (<<SRC: fsem_src varg = resum_itr itr_src>>) /\ *)
+(*           (<<TGT: fsem_tgt varg = resum_itr itr_tgt>>) /\ *)
+(*           (<<SIM: exists i0, simg i0 itr_src itr_tgt>>)>>) *)
+(* . *)
+(* Hypothesis (SIM: Forall2 sim_fnsem ms_src.(ModSem.fnsems) ms_tgt.(ModSem.fnsems)). *)
 
-Hypothesis (SIM: Forall2 sim_fnsem ms_src.(ModSem.fnsems) ms_tgt.(ModSem.fnsems)).
+Hypothesis (SIM: exists o0, simg o0 (ModSem.initial_itr ms_src) (ModSem.initial_itr ms_tgt)).
 
 Theorem adequacy_global: Beh.of_program (Mod.interp md_tgt) <1= Beh.of_program (Mod.interp md_src).
 Proof.
